Misc/Int.lean
@@ -1,16 +1,6 @@
 namespace Int
   variable (n m o : Int)
 
-  theorem min_assoc : min (min n m) o = min n (min m o) := by
-    repeat rw [Int.min_def]
-    repeat' split
-    all_goals omega
-
-  theorem max_assoc : max (max n m) o = max n (max m o) := by
-    repeat rw [Int.max_def]
-    repeat' split
-    all_goals omega
-
   theorem min_max_absorb : min n (max n m) = n := by
     apply Int.min_eq_left
     apply Int.le_max_left
