Misc/Vector.lean
@@ -4,7 +4,7 @@ namespace Batteries.Vector
 
 /-- Map a monadic function over a vector. -/
 def mapM {α β m} [Monad m] (f : α → m β) {n} (v : Vector α n) : m (Vector β n) := do
-  go 0 (Nat.zero_le n) .empty
+  go 0 (Nat.zero_le n) (.emptyWithCapacity n)
 where
   go (i : Nat) (h : i ≤ n) (r : Vector β i) : m (Vector β n) := do
     if h' : i < n then
@@ -13,31 +13,28 @@ where
       return r.cast (by omega)
 
 @[simp]
-theorem get_mk_vector_fin {α n} : ∀ (x : α) (i : Fin n), (mkVector n x).get i = x := by
+theorem get_mk_vector_fin {α n} : ∀ (x : α) (i : Fin n), (Vector.replicate n x).get i = x := by
   intros x i
-  show (mkArray n x)[i] = x
-  simp [mkArray]
+  apply Vector.getElem_replicate
 
 @[simp]
-theorem get_mk_vector_nat {α n} : ∀ (x : α) (i : Nat) (h : i < n), (mkVector n x)[i] = x := by
+theorem get_mk_vector_nat {α n} : ∀ (x : α) (i : Nat) (h : i < n), (Vector.replicate  n x)[i] = x := by
   intros x i h
-  simp [mkVector]
-  have : i < (mkArray n x).size := by simpa using h
-  show (mkArray n x)[i] = x
-  simp [mkArray]
+  rw [Vector.replicate]
+  have : i < (Vector.replicate n x).size := by simpa using h
+  show (Vector.replicate n x)[i] = x
+  simp
 
 @[simp]
-theorem get_of_fn_fin {α n} : ∀ (f : Fin n → α) (i : Fin n), (ofFn f).get i = f i := by
+theorem get_of_fn_fin {α n} : ∀ (f : Fin n → α) (i : Fin n), (Vector.ofFn f).get i = f i := by
   intros f i
-  simp [ofFn]
+  simp [Vector.ofFn]
   show (Array.ofFn f)[i] = f i
   simp
 
 @[simp]
-theorem get_of_fn_nat {α n} : ∀ (f : Fin n → α) (i : Nat) (h : i < n), (ofFn f)[i] = f ⟨i, h⟩ := by
+theorem get_of_fn_nat {α n} : ∀ (f : Fin n → α) (i : Nat) (h : i < n), (Vector.ofFn f)[i] = f ⟨i, h⟩ := by
   intros f i h
-  simp [ofFn]
-  have : i < (Array.ofFn f).size := by simpa using h
-  show (Array.ofFn f)[i] = f ⟨i, h⟩
-  simp
+  simp [Vector.ofFn]
+
 end Batteries.Vector
