lakefile.lean
@@ -1,9 +1,9 @@
 import Lake
 open Lake DSL
 
-require batteries from git "https://github.com/leanprover-community/batteries" @ "v4.12.0"
+require batteries from git "https://github.com/leanprover-community/batteries" @ "v4.24.0"
 
-require aesop from git "https://github.com/leanprover-community/aesop" @ "v4.12.0"
+require aesop from git "https://github.com/leanprover-community/aesop" @ "v4.24.0"
 
 package "lustrean" where
   version := v!"0.1.0"
